code/nist-pcurves/Hacl.Impl.PCurves.Constants.fst
@@ -15,147 +15,58 @@ module SM = Hacl.Spec.PCurves.Montgomery
 
 #set-options "--z3rlimit 50 --fuel 0 --ifuel 0"
 
-val make_prime: {| cp:S.curve_params |} -> n:felem -> Stack unit
+let fmont_as_nat {| S.curve_params |} (h:mem) (a:felem) = SM.from_mont (as_nat h a)
+
+let qmont_as_nat {| c:S.curve_params |} (h:mem) (a:felem) = SM.from_qmont (as_nat h a)
+
+
+class curve_constants {| cp:S.curve_params |} = {
+  make_prime : n:felem -> Stack unit
   (requires fun h -> live h n)
   (ensures  fun h0 _ h1 -> modifies (loc n) h0 h1 /\
-    as_nat h1 n == S.prime)
-
-[@CInline]
-let make_prime {| cp:S.curve_params |} n =
-  if cp.bn_limbs = 4ul then (
-    assume (cp.prime == Spec.P256.p256_prime);
-    // 0xffffffff00000001000000000000000000000000ffffffffffffffffffffffff
-    [@inline_let] let n0 = u64 0xffffffffffffffff in
-    [@inline_let] let n1 = u64 0xffffffff in
-    [@inline_let] let n2 = u64 0x0 in
-    [@inline_let] let n3 = u64 0xffffffff00000001 in
-    assert_norm (v n0 + v n1 * pow2 64 + v n2 * pow2 128 + v n3 * pow2 192 = Spec.P256.p256_prime);
-    bn_make_u64_4 n n0 n1 n2 n3)
-  else admit()
-
-
-val make_order: {| cp:S.curve_params |} -> n:felem -> Stack unit
+    as_nat h1 n == cp.prime);
+  make_order: n:felem -> Stack unit
   (requires fun h -> live h n)
   (ensures  fun h0 _ h1 -> modifies (loc n) h0 h1 /\
-    as_nat h1 n == S.order)
-
-[@CInline]
-let make_order {| cp:S.curve_params |} n =
-  if cp.bn_limbs = 4ul then (
-    assume (cp.order = Spec.P256.p256_order);
-    // 0xffffffff00000000ffffffffffffffffbce6faada7179e84f3b9cac2fc632551
-    [@inline_let] let n0 = u64 0xf3b9cac2fc632551 in
-    [@inline_let] let n1 = u64 0xbce6faada7179e84 in
-    [@inline_let] let n2 = u64 0xffffffffffffffff in
-    [@inline_let] let n3 = u64 0xffffffff00000000 in
-    assert_norm (v n0 + v n1 * pow2 64 + v n2 * pow2 128 + v n3 * pow2 192 = Spec.P256.p256_order);
-    bn_make_u64_4 n n0 n1 n2 n3)
-  else admit()
-
-val make_a_coeff: {| cp:S.curve_params |} -> a:felem -> Stack unit
+    as_nat h1 n == S.order);
+  make_a_coeff: a:felem -> Stack unit
   (requires fun h -> live h a)
   (ensures fun h0 _ h1 -> modifies (loc a) h0 h1 /\
     as_nat h1 a < S.prime /\
-    SM.from_mont (as_nat h1 a) == S.a_coeff)
-
-[@CInline]
-let make_a_coeff {| cp:S.curve_params |} a =
-  if cp.bn_limbs = 4ul then (
-    admit();
-    // a_coeff      = 0xffffffff00000001000000000000000000000000fffffffffffffffffffffffc
-    // a_coeff_mont = 0xfffffffc00000004000000000000000000000003fffffffffffffffffffffffc
-    [@inline_let] let n0 = u64 0xfffffffffffffffc in
-    [@inline_let] let n1 = u64 0x3ffffffff in
-    [@inline_let] let n2 = u64 0x0 in
-    [@inline_let] let n3 = u64 0xfffffffc00000004 in
-    assert_norm (v n0 + v n1 * pow2 64 + v n2 * pow2 128 + v n3 * pow2 192 < S.prime);
-    assert_norm (SM.to_mont S.a_coeff == v n0 + v n1 * pow2 64 + v n2 * pow2 128 + v n3 * pow2 192);
-    SM.lemma_to_from_mont_id S.a_coeff;
-    bn_make_u64_4 a n0 n1 n2 n3 )
-  else admit()
-
-val make_b_coeff: {| cp:S.curve_params |} -> b:felem -> Stack unit
+    SM.from_mont (as_nat h1 a) == S.a_coeff);
+  make_b_coeff: b:felem -> Stack unit
   (requires fun h -> live h b)
   (ensures fun h0 _ h1 -> modifies (loc b) h0 h1 /\
     as_nat h1 b < S.prime /\
-    SM.from_mont (as_nat h1 b) == S.b_coeff)
-
-[@CInline]
-let make_b_coeff {| cp:S.curve_params |} b =
-  if cp.bn_limbs = 4ul then (
-    admit();
-    // b_coeff      = 0x5ac635d8aa3a93e7b3ebbd55769886bc651d06b0cc53b0f63bce3c3e27d2604b
-    // b_coeff_mont = 0xdc30061d04874834e5a220abf7212ed6acf005cd78843090d89cdf6229c4bddf
-    [@inline_let] let n0 = u64 0xd89cdf6229c4bddf in
-    [@inline_let] let n1 = u64 0xacf005cd78843090 in
-    [@inline_let] let n2 = u64 0xe5a220abf7212ed6 in
-    [@inline_let] let n3 = u64 0xdc30061d04874834 in
-    assert_norm (v n0 + v n1 * pow2 64 + v n2 * pow2 128 + v n3 * pow2 192 < S.prime);
-    assert_norm (SM.to_mont S.b_coeff == v n0 + v n1 * pow2 64 + v n2 * pow2 128 + v n3 * pow2 192);
-    SM.lemma_to_from_mont_id S.b_coeff;
-    bn_make_u64_4 b n0 n1 n2 n3)
-  else admit()
-
-
-val make_g_x: {| cp:S.curve_params |} -> n:felem -> Stack unit
+    SM.from_mont (as_nat h1 b) == S.b_coeff);
+  make_g_x: n:felem -> Stack unit
   (requires fun h -> live h n)
   (ensures  fun h0 _ h1 -> modifies (loc n) h0 h1 /\
     as_nat h1 n < S.prime /\
-    SM.from_mont (as_nat h1 n) == S.basepoint_x)
-
-[@CInline]
-let make_g_x {| cp:S.curve_params |} n =
-  admit();
-  if cp.bn_limbs = 4ul then
-    // g_x = 0x6b17d1f2e12c4247f8bce6e563a440f277037d812deb33a0f4a13945d898c296
-    // mont_g_x = 0x18905f76a53755c679fb732b7762251075ba95fc5fedb60179e730d418a9143c
-    [@inline_let] let n0 = u64 0x79e730d418a9143c in
-    [@inline_let] let n1 = u64 0x75ba95fc5fedb601 in
-    [@inline_let] let n2 = u64 0x79fb732b77622510 in
-    [@inline_let] let n3 = u64 0x18905f76a53755c6 in
-    assert_norm (v n0 + v n1 * pow2 64 + v n2 * pow2 128 + v n3 * pow2 192 < S.prime);
-    assert_norm (SM.to_mont S.basepoint_x == v n0 + v n1 * pow2 64 + v n2 * pow2 128 + v n3 * pow2 192);
-    SM.lemma_to_from_mont_id S.basepoint_x;
-    bn_make_u64_4 n n0 n1 n2 n3
-  else admit()
-
-val make_g_y: {| cp:S.curve_params |} -> n:felem -> Stack unit
+    SM.from_mont (as_nat h1 n) == S.basepoint_x);
+  make_g_y: n:felem -> Stack unit
   (requires fun h -> live h n)
   (ensures  fun h0 _ h1 -> modifies (loc n) h0 h1 /\
     as_nat h1 n < S.prime /\
-    SM.from_mont (as_nat h1 n) == S.basepoint_y)
-
-[@CInline]
-let make_g_y {| cp:S.curve_params |} n =
-  admit();
-  if cp.bn_limbs = 4ul then
-    // g_y = 0x4fe342e2fe1a7f9b8ee7eb4a7c0f9e162bce33576b315ececbb6406837bf51f5
-    // mont_g_x = 0x8571ff1825885d85d2e88688dd21f3258b4ab8e4ba19e45cddf25357ce95560a
-    [@inline_let] let n0 = u64 0xddf25357ce95560a in
-    [@inline_let] let n1 = u64 0x8b4ab8e4ba19e45c in
-    [@inline_let] let n2 = u64 0xd2e88688dd21f325 in
-    [@inline_let] let n3 = u64 0x8571ff1825885d85 in
-    assert_norm (v n0 + v n1 * pow2 64 + v n2 * pow2 128 + v n3 * pow2 192 < S.prime);
-    assert_norm (SM.to_mont S.basepoint_y == v n0 + v n1 * pow2 64 + v n2 * pow2 128 + v n3 * pow2 192);
-    SM.lemma_to_from_mont_id S.basepoint_y;
-    bn_make_u64_4 n n0 n1 n2 n3
-  else admit()
-
-val make_fmont_R2: {| cp:S.curve_params |} -> n:felem -> Stack unit
+    SM.from_mont (as_nat h1 n) == S.basepoint_y);
+  make_fmont_R2: n:felem -> Stack unit
   (requires fun h -> live h n)
   (ensures  fun h0 _ h1 -> modifies (loc n) h0 h1 /\
-    as_nat h1 n == SM.fmont_R * SM.fmont_R % S.prime)
-
-[@CInline]
-let make_fmont_R2 {| cp:S.curve_params |}n =
-  admit();
-  if cp.bn_limbs = 4ul then 
-    // 0x4fffffffdfffffffffffffffefffffffbffffffff0000000000000003
-    [@inline_let] let n0 = u64 0x3 in
-    [@inline_let] let n1 = u64 0xfffffffbffffffff in
-    [@inline_let] let n2 = u64 0xfffffffffffffffe in
-    [@inline_let] let n3 = u64 0x4fffffffd in
-    assert_norm (v n0 + v n1 * pow2 64 + v n2 * pow2 128 + v n3 * pow2 192 ==
-      SM.fmont_R * SM.fmont_R % S.prime);
-    bn_make_u64_4 n n0 n1 n2 n3
-  else admit()
+    as_nat h1 n == SM.fmont_R * SM.fmont_R % S.prime);
+  make_fzero: n:felem -> Stack unit
+  (requires fun h -> live h n)
+  (ensures  fun h0 _ h1 -> modifies (loc n) h0 h1 /\
+    as_nat h1 n < S.prime /\
+    fmont_as_nat h1 n == 0);
+  make_fone: n:felem -> Stack unit
+  (requires fun h -> live h n)
+  (ensures  fun h0 _ h1 -> modifies (loc n) h0 h1 /\
+    as_nat h1 n < S.prime /\
+    fmont_as_nat h1 n == 1);
+  make_qone: f:felem -> Stack unit
+  (requires fun h -> live h f)
+  (ensures  fun h0 _ h1 -> modifies (loc f) h0 h1 /\
+    as_nat h1 f < S.order /\
+    qmont_as_nat h1 f == 1)
+}
+  
