code/nist-pcurves/Hacl.Impl.PCurves.Field.fsti
@@ -12,31 +12,14 @@ open Hacl.Impl.PCurves.Bignum
 
 module S = Spec.PCurves
 module SM = Hacl.Spec.PCurves.Montgomery
+module CC = Hacl.Impl.PCurves.Constants
 
 #set-options "--z3rlimit 50 --fuel 0 --ifuel 0"
 
-let fmont_as_nat {| S.curve_params |} (h:mem) (a:felem) = SM.from_mont (as_nat h a)
-
-
-///  Create zero and one
-
-val make_fzero: {| S.curve_params |} -> n:felem -> Stack unit
-  (requires fun h -> live h n)
-  (ensures  fun h0 _ h1 -> modifies (loc n) h0 h1 /\
-    as_nat h1 n < S.prime /\
-    fmont_as_nat h1 n == 0)
-
-
-val make_fone: {| S.curve_params |} -> n:felem -> Stack unit
-  (requires fun h -> live h n)
-  (ensures  fun h0 _ h1 -> modifies (loc n) h0 h1 /\
-    as_nat h1 n < S.prime /\
-    fmont_as_nat h1 n == 1)
-
-
 ///  Comparison
 
-val bn_is_lt_prime_mask: {| S.curve_params |} -> f:felem -> Stack uint64
+val bn_is_lt_prime_mask {| S.curve_params |} {| CC.curve_constants |}:
+    f:felem -> Stack uint64
   (requires fun h -> live h f)
   (ensures  fun h0 r h1 -> modifies0 h0 h1 /\
     (if as_nat h0 f < S.prime then v r = ones_v U64 else v r = 0))
@@ -47,75 +30,83 @@ val feq_mask: {| S.curve_params |} -> a:felem -> b:felem -> Stack uint64
     live h a /\ live h b /\ eq_or_disjoint a b /\
     as_nat h a < S.prime /\ as_nat h b < S.prime)
   (ensures fun h0 r h1 -> modifies0 h0 h1 /\
-    (if fmont_as_nat h0 a = fmont_as_nat h0 b then v r == ones_v U64 else v r = 0))
+    (if CC.fmont_as_nat h0 a = CC.fmont_as_nat h0 b then v r == ones_v U64 else v r = 0))
 
 
 ///  Field Arithmetic
 
-val fadd: {| S.curve_params |} -> res:felem -> x:felem -> y:felem -> Stack unit
+val fadd {| S.curve_params |} {| CC.curve_constants |}:
+  res:felem -> x:felem -> y:felem -> Stack unit
   (requires fun h ->
     live h x /\ live h y /\ live h res /\
     eq_or_disjoint x y /\ eq_or_disjoint x res /\ eq_or_disjoint y res /\
     as_nat h x < S.prime /\ as_nat h y < S.prime)
   (ensures  fun h0 _ h1 -> modifies (loc res) h0 h1 /\
     as_nat h1 res == S.fadd (as_nat h0 x) (as_nat h0 y) /\
-    fmont_as_nat h1 res == S.fadd (fmont_as_nat h0 x) (fmont_as_nat h0 y))
+    CC.fmont_as_nat h1 res == S.fadd (CC.fmont_as_nat h0 x) (CC.fmont_as_nat h0 y))
 
 
 inline_for_extraction noextract
-val fdouble: {| S.curve_params |} -> res:felem -> x:felem -> Stack unit
+val fdouble {| S.curve_params |} {| CC.curve_constants |}:
+  res:felem -> x:felem -> Stack unit
   (requires fun h ->
     live h x /\ live h res /\ eq_or_disjoint x res /\
     as_nat h x < S.prime)
   (ensures fun h0 _ h1 -> modifies (loc res) h0 h1 /\
     as_nat h1 res == (2 * as_nat h0 x) % S.prime /\
-    fmont_as_nat h1 res == (2 * fmont_as_nat h0 x) % S.prime)
+    CC.fmont_as_nat h1 res == (2 * CC.fmont_as_nat h0 x) % S.prime)
 
 
-val fsub: {| S.curve_params |} -> res:felem -> x:felem -> y:felem -> Stack unit
+val fsub {| S.curve_params |} {| CC.curve_constants |}:
+  res:felem -> x:felem -> y:felem -> Stack unit
   (requires fun h ->
     live h res /\ live h x /\ live h y /\
     eq_or_disjoint x y /\ eq_or_disjoint x res /\ eq_or_disjoint y res /\
     as_nat h x < S.prime /\ as_nat h y < S.prime)
   (ensures fun h0 _ h1 -> modifies (loc res) h0 h1 /\
     as_nat h1 res == S.fsub (as_nat h0 x) (as_nat h0 y) /\
-    fmont_as_nat h1 res == S.fsub (fmont_as_nat h0 x) (fmont_as_nat h0 y))
+    CC.fmont_as_nat h1 res == S.fsub (CC.fmont_as_nat h0 x) (CC.fmont_as_nat h0 y))
 
 
-val fnegate_conditional_vartime: {| S.curve_params |} -> f:felem -> is_negate:bool -> Stack unit
+val fnegate_conditional_vartime {| S.curve_params |} {| CC.curve_constants |}:
+  f:felem -> is_negate:bool -> Stack unit
   (requires fun h -> live h f /\ as_nat h f < S.prime)
   (ensures  fun h0 _ h1 -> modifies (loc f) h0 h1 /\ as_nat h1 f < S.prime /\
     as_nat h1 f == (if is_negate then (S.prime - as_nat h0 f) % S.prime else as_nat h0 f))
 
 
-val fmul: {| S.curve_params |} -> res:felem -> x:felem -> y:felem -> Stack unit
+val fmul {| S.curve_params |} {| CC.curve_constants |}:
+  res:felem -> x:felem -> y:felem -> Stack unit
   (requires fun h ->
     live h x /\ live h y /\ live h res /\
     eq_or_disjoint x y /\ eq_or_disjoint x res /\ eq_or_disjoint y res /\
     as_nat h x < S.prime /\ as_nat h y < S.prime)
   (ensures fun h0 _ h1 -> modifies (loc res) h0 h1 /\
     as_nat h1 res = (as_nat h0 x * as_nat h0 y * SM.fmont_R_inv) % S.prime /\
-    fmont_as_nat h1 res = S.fmul (fmont_as_nat h0 x) (fmont_as_nat h0 y))
+    CC.fmont_as_nat h1 res = S.fmul (CC.fmont_as_nat h0 x) (CC.fmont_as_nat h0 y))
 
 
-val fsqr: {| S.curve_params |} -> res:felem -> x:felem -> Stack unit
+val fsqr {| S.curve_params |} {| CC.curve_constants |}:
+  res:felem -> x:felem -> Stack unit
   (requires fun h ->
     live h x /\ live h res /\ eq_or_disjoint x res /\
     as_nat h x < S.prime)
   (ensures  fun h0 _ h1 -> modifies (loc res) h0 h1 /\
     as_nat h1 res = (as_nat h0 x * as_nat h0 x * SM.fmont_R_inv) % S.prime /\
-    fmont_as_nat h1 res = S.fmul (fmont_as_nat h0 x) (fmont_as_nat h0 x))
+    CC.fmont_as_nat h1 res = S.fmul (CC.fmont_as_nat h0 x) (CC.fmont_as_nat h0 x))
 
 
-val from_mont: {| S.curve_params |} -> res:felem -> x:felem -> Stack unit
+val from_mont {| S.curve_params |} {| CC.curve_constants |}:
+  res:felem -> x:felem -> Stack unit
   (requires fun h ->
     live h x /\ live h res /\ as_nat h x < S.prime)
   (ensures  fun h0 _ h1 -> modifies (loc res) h0 h1 /\
     as_nat h1 res = (as_nat h0 x * SM.fmont_R_inv) % S.prime /\
-    as_nat h1 res = fmont_as_nat h0 x)
+    as_nat h1 res = CC.fmont_as_nat h0 x)
 
 
-val to_mont: {| S.curve_params |} -> res:felem -> f:felem -> Stack unit
+val to_mont {| S.curve_params |} {| CC.curve_constants |}:
+  res:felem -> f:felem -> Stack unit
   (requires fun h ->
     live h f /\ live h res /\ eq_or_disjoint f res /\
     as_nat h f < S.prime)
@@ -125,21 +116,23 @@ val to_mont: {| S.curve_params |} -> res:felem -> f:felem -> Stack unit
 
 ///  Special cases of the above functions
 
-val fmul_by_b_coeff: {| S.curve_params |} -> res:felem -> x:felem -> Stack unit
+val fmul_by_b_coeff {| S.curve_params |} {| CC.curve_constants |}:
+  res:felem -> x:felem -> Stack unit
   (requires fun h ->
     live h x /\ live h res /\ eq_or_disjoint x res /\
     as_nat h x < S.prime)
   (ensures fun h0 _ h1 -> modifies (loc res) h0 h1 /\
     as_nat h1 res < S.prime /\
-    fmont_as_nat h1 res =
-      S.fmul S.b_coeff (fmont_as_nat h0 x))
+    CC.fmont_as_nat h1 res =
+      S.fmul S.b_coeff (CC.fmont_as_nat h0 x))
 
 
-val fcube: {| S.curve_params |} -> res:felem -> x:felem -> Stack unit
+val fcube {| S.curve_params |} {| CC.curve_constants |}:
+  res:felem -> x:felem -> Stack unit
   (requires fun h ->
     live h x /\ live h res /\ disjoint x res /\
     as_nat h x < S.prime)
   (ensures fun h0 _ h1 -> modifies (loc res) h0 h1 /\
     as_nat h1 res < S.prime /\
-    fmont_as_nat h1 res =
-      S.fmul (S.fmul (fmont_as_nat h0 x) (fmont_as_nat h0 x)) (fmont_as_nat h0 x))
+    CC.fmont_as_nat h1 res =
+      S.fmul (S.fmul (CC.fmont_as_nat h0 x) (CC.fmont_as_nat h0 x)) (CC.fmont_as_nat h0 x))
