code/nist-pcurves/Hacl.Impl.PCurves.PointMul.fst
@@ -28,7 +28,7 @@ module PP = Hacl.PCurves.PrecompTable
 #set-options "--z3rlimit 50 --fuel 0 --ifuel 0"
 
 inline_for_extraction noextract
-let table_inv_w4 {| cp:S.curve_params |} : BE.table_inv_t U64 (3ul *. cp.bn_limbs) 16ul =
+let table_inv_w4 {| cp:S.curve_params |} {| curve_constants |} {| curve_inv_sqrt |} : BE.table_inv_t U64 (3ul *. cp.bn_limbs) 16ul =
   [@inline_let] let len = 3ul *. cp.bn_limbs in
   [@inline_let] let ctx_len = 0ul in
   [@inline_let] let k = mk_pcurve_concrete_ops in
@@ -38,7 +38,7 @@ let table_inv_w4 {| cp:S.curve_params |} : BE.table_inv_t U64 (3ul *. cp.bn_limb
 
 
 inline_for_extraction noextract
-let table_inv_w5 {| cp:S.curve_params |} : BE.table_inv_t U64 (3ul *. cp.bn_limbs) 32ul =
+let table_inv_w5 {| cp:S.curve_params |} {| curve_constants |} {| curve_inv_sqrt |} : BE.table_inv_t U64 (3ul *. cp.bn_limbs) 32ul =
   [@inline_let] let len = 3ul *. cp.bn_limbs in
   [@inline_let] let ctx_len = 0ul in
   [@inline_let] let k = mk_pcurve_concrete_ops in
@@ -49,7 +49,7 @@ let table_inv_w5 {| cp:S.curve_params |} : BE.table_inv_t U64 (3ul *. cp.bn_limb
 
 
 [@CInline]
-let point_mul {| cp:S.curve_params |} res scalar p =
+let point_mul {| cp:S.curve_params |} {| curve_constants |} {| curve_inv_sqrt |} res scalar p =
   let h0 = ST.get () in
   SE.exp_fw_lemma S.mk_pcurve_concrete_ops
     (from_mont_point (as_point_nat h0 p)) cp.bits (as_nat h0 scalar) (v cp.bn_limbs);
@@ -58,10 +58,10 @@ let point_mul {| cp:S.curve_params |} res scalar p =
   BE.lexp_fw_consttime (3ul *. cp.bn_limbs) 0ul mk_pcurve_concrete_ops (cp.bn_limbs) (null uint64) p cp.bn_limbs (size cp.bits) scalar res
 
 
-val precomp_get_consttime {| cp:S.curve_params |} : BE.pow_a_to_small_b_st U64 (3ul *. cp.bn_limbs) 0ul mk_pcurve_concrete_ops 4ul 16ul
+val precomp_get_consttime {| cp:S.curve_params |} {| curve_constants |} {| curve_inv_sqrt |} : BE.pow_a_to_small_b_st U64 (3ul *. cp.bn_limbs) 0ul mk_pcurve_concrete_ops 4ul 16ul
     (BE.table_inv_precomp (3ul *. cp.bn_limbs) 0ul mk_pcurve_concrete_ops 4ul 16ul)
 [@CInline]
-let precomp_get_consttime {| cp:S.curve_params |} ctx a table bits_l tmp =
+let precomp_get_consttime {| cp:S.curve_params |} {| curve_constants |} {| curve_inv_sqrt |} ctx a table bits_l tmp =
   [@inline_let] let len = 3ul *. cp.bn_limbs in
   [@inline_let] let ctx_len = 0ul in
   [@inline_let] let k = mk_pcurve_concrete_ops in
@@ -72,7 +72,7 @@ let precomp_get_consttime {| cp:S.curve_params |} ctx a table bits_l tmp =
 
 
 inline_for_extraction noextract
-val point_mul_g_noalloc {| cp:S.curve_params |} {| pt:precomp_tables |}
+val point_mul_g_noalloc {| cp:S.curve_params |} {| curve_constants |} {| curve_inv_sqrt |} {| pt:precomp_tables |}
   : out:point -> scalar:felem
   -> q1:point -> q2:point
   -> q3:point -> q4:point ->
@@ -96,7 +96,7 @@ val point_mul_g_noalloc {| cp:S.curve_params |} {| pt:precomp_tables |}
     S.to_aff_point (from_mont_point (as_point_nat h1 out)) ==
     LE.exp_four_fw S.mk_pcurve_comm_monoid g_aff 64 b0 g_pow2_64 b1 g_pow2_128 b2 g_pow2_192 b3 4))
 
-let point_mul_g_noalloc {| cp:S.curve_params |} {| pt:precomp_tables |} out scalar q1 q2 q3 q4 =
+let point_mul_g_noalloc {| cp:S.curve_params |} {| curve_constants |} {| curve_inv_sqrt |} {| pt:precomp_tables |} out scalar q1 q2 q3 q4 =
   [@inline_let] let len = 3ul *. cp.bn_limbs in
   [@inline_let] let ctx_len = 0ul in
   [@inline_let] let k = mk_pcurve_concrete_ops in
@@ -148,13 +148,13 @@ let point_mul_g_noalloc {| cp:S.curve_params |} {| pt:precomp_tables |} out scal
     out
 
 
-val lemma_exp_four_fw_local {| cp:S.curve_params |}: b:BD.lbignum U64 4{BD.bn_v b < S.order} ->
+val lemma_exp_four_fw_local {| cp:S.curve_params |} {| curve_constants |} {| curve_inv_sqrt |} : b:BD.lbignum U64 4{BD.bn_v b < S.order} ->
   Lemma (cp.bits == 256 ==> (
     let (b0, b1, b2, b3) = SPT256.decompose_nat256_as_four_u64 (BD.bn_v b) in
     LE.exp_four_fw S.mk_pcurve_comm_monoid g_aff 64 b0 g_pow2_64 b1 g_pow2_128 b2 g_pow2_192 b3 4 ==
     S.to_aff_point (S.point_mul_g (BD.bn_v b))))
 
-let lemma_exp_four_fw_local {| cp:S.curve_params |} b =
+let lemma_exp_four_fw_local {| cp:S.curve_params |} {| curve_constants |} {| curve_inv_sqrt |} b =
   let cm = S.mk_pcurve_comm_monoid in
   admit();
   let (b0, b1, b2, b3) = SPT256.decompose_nat256_as_four_u64 (BD.bn_v b) in
@@ -168,7 +168,7 @@ let lemma_exp_four_fw_local {| cp:S.curve_params |} b =
 
 
 [@CInline]
-let point_mul_g {| cp:S.curve_params |} {| pt:precomp_tables |}  res scalar =
+let point_mul_g {| cp:S.curve_params |} {| curve_constants |} {| curve_inv_sqrt |} {| pt:precomp_tables |}  res scalar =
   push_frame ();
   let h0 = ST.get () in
   let q1 = create_point #cp in
@@ -191,7 +191,7 @@ let point_mul_g {| cp:S.curve_params |} {| pt:precomp_tables |}  res scalar =
 //-------------------------
 
 inline_for_extraction noextract
-val point_mul_g_double_vartime_noalloc {| cp:S.curve_params |} {| pt:precomp_tables |} :
+val point_mul_g_double_vartime_noalloc {| cp:S.curve_params |} {| curve_constants |} {| curve_inv_sqrt |} {| pt:precomp_tables |} :
     out:point
   -> scalar1:felem -> q1:point
   -> scalar2:felem -> q2:point
@@ -213,7 +213,7 @@ val point_mul_g_double_vartime_noalloc {| cp:S.curve_params |} {| pt:precomp_tab
     S.to_aff_point (S.point_mul_double_g
       (as_nat h0 scalar1) (as_nat h0 scalar2) (from_mont_point (as_point_nat h0 q2))))
 
-let point_mul_g_double_vartime_noalloc {| cp:S.curve_params |} {| pt:precomp_tables |} out scalar1 q1 scalar2 q2 table2 =
+let point_mul_g_double_vartime_noalloc {| cp:S.curve_params |} {| curve_constants |} {| curve_inv_sqrt |} {| pt:precomp_tables |} out scalar1 q1 scalar2 q2 table2 =
   [@inline_let] let len = 3ul *. cp.bn_limbs in
   [@inline_let] let ctx_len = 0ul in
   [@inline_let] let k = mk_pcurve_concrete_ops in
@@ -243,7 +243,7 @@ let point_mul_g_double_vartime_noalloc {| cp:S.curve_params |} {| pt:precomp_tab
 
 
 [@CInline]
-let point_mul_double_g {| cp:S.curve_params |} {| pt:precomp_tables |} res scalar1 scalar2 q2 =
+let point_mul_double_g {| cp:S.curve_params |} {| curve_constants |} {| curve_inv_sqrt |} {| pt:precomp_tables |} res scalar1 scalar2 q2 =
   push_frame ();
   [@inline_let] let len = 3ul *. cp.bn_limbs in
   [@inline_let] let ctx_len = 0ul in
