code/nist-pcurves/Hacl.Impl.PCurves.Sign.fst
@@ -9,6 +9,8 @@ open Lib.IntTypes
 open Lib.Buffer
 
 open Hacl.Impl.PCurves.Bignum
+open Hacl.Impl.PCurves.Constants
+open Hacl.Impl.PCurves.InvSqrt
 open Hacl.Impl.PCurves.Scalar
 open Hacl.Impl.PCurves.Point
 open Hacl.Impl.PCurves.PointMul
@@ -27,7 +29,7 @@ inline_for_extraction noextract
 let lbytes len = lbuffer uint8 len
 
 inline_for_extraction noextract
-val ecdsa_sign_r  {| cp:S.curve_params |} {| PP.precomp_tables |} (r k:felem) : Stack unit
+val ecdsa_sign_r  {| cp:S.curve_params |} {| curve_constants |} {| curve_inv_sqrt |} {| PP.precomp_tables |} (r k:felem) : Stack unit
   (requires fun h ->
     live h r /\ live h k /\ disjoint r k /\
     as_nat h k < S.order)
@@ -35,7 +37,7 @@ val ecdsa_sign_r  {| cp:S.curve_params |} {| PP.precomp_tables |} (r k:felem) : 
    (let x, _ = S.to_aff_point (S.point_mul_g (as_nat h0 k)) in
     as_nat h1 r == x % S.order))
 
-let ecdsa_sign_r {| cp:S.curve_params |} {| PP.precomp_tables |} r k =
+let ecdsa_sign_r {| cp:S.curve_params |} {| curve_constants |} {| curve_inv_sqrt |} {| PP.precomp_tables |} r k =
   push_frame ();
   let p = create_point #cp in
   point_mul_g p k; // p = [k]G
@@ -45,7 +47,7 @@ let ecdsa_sign_r {| cp:S.curve_params |} {| PP.precomp_tables |} r k =
 
 
 inline_for_extraction noextract
-val ecdsa_sign_s {| cp:S.curve_params |} {| PP.precomp_tables |} (s k r d_a m:felem) : Stack unit
+val ecdsa_sign_s {| cp:S.curve_params |} {| curve_constants |} {| curve_inv_sqrt |} {| PP.precomp_tables |} (s k r d_a m:felem) : Stack unit
   (requires fun h ->
     live h s /\ live h m /\ live h d_a /\ live h k /\ live h r /\
     disjoint s r /\ disjoint s k /\ disjoint r k /\
@@ -58,11 +60,11 @@ val ecdsa_sign_s {| cp:S.curve_params |} {| PP.precomp_tables |} (s k r d_a m:fe
    (let kinv = S.qinv (as_nat h0 k) in
     as_nat h1 s == S.qmul kinv (S.qadd (as_nat h0 m) (S.qmul (as_nat h0 r) (as_nat h0 d_a)))))
 
-let ecdsa_sign_s {| cp:S.curve_params |} {| PP.precomp_tables |} s k r d_a m =
+let ecdsa_sign_s {| cp:S.curve_params |} {| curve_constants |} {| curve_inv_sqrt |} {| PP.precomp_tables |} s k r d_a m =
   push_frame ();
   let h0 = ST.get () in
   let kinv = create_felem #cp in
-  QI.qinv kinv k;
+  qinv kinv k;
   let h1 = ST.get () in
   assert (qmont_as_nat h1 kinv == S.qinv (qmont_as_nat h0 k));
   SM.qmont_inv_lemma (as_nat h0 k);
@@ -86,7 +88,7 @@ let ecdsa_sign_s {| cp:S.curve_params |} {| PP.precomp_tables |} s k r d_a m =
 
 
 inline_for_extraction noextract
-val ecdsa_sign_load {| cp:S.curve_params |} {| PP.precomp_tables |} (d_a k_q:felem) (private_key nonce:lbytes (size cp.bytes)) : Stack uint64
+val ecdsa_sign_load {| cp:S.curve_params |} {| curve_constants |} {| curve_inv_sqrt |} {| PP.precomp_tables |} (d_a k_q:felem) (private_key nonce:lbytes (size cp.bytes)) : Stack uint64
   (requires fun h ->
     live h private_key /\ live h nonce /\ live h d_a /\ live h k_q /\
     disjoint d_a k_q /\ disjoint d_a private_key /\ disjoint d_a nonce /\
@@ -101,7 +103,7 @@ val ecdsa_sign_load {| cp:S.curve_params |} {| PP.precomp_tables |} (d_a k_q:fel
     as_nat h1 d_a == (if is_sk_valid then d_a_nat else 1) /\
     as_nat h1 k_q == (if is_nonce_valid then k_nat else 1)))
 
-let ecdsa_sign_load {| cp:S.curve_params |} {| PP.precomp_tables |} d_a k_q private_key nonce =
+let ecdsa_sign_load {| cp:S.curve_params |} {| curve_constants |} {| curve_inv_sqrt |} {| PP.precomp_tables |} d_a k_q private_key nonce =
   let is_sk_valid = load_qelem_conditional d_a private_key in
   let is_nonce_valid = load_qelem_conditional k_q nonce in
   let m = is_sk_valid &. is_nonce_valid in
@@ -110,14 +112,15 @@ let ecdsa_sign_load {| cp:S.curve_params |} {| PP.precomp_tables |} d_a k_q priv
 
 
 inline_for_extraction noextract
-val check_signature: {| cp:S.curve_params |} -> {| PP.precomp_tables |} -> are_sk_nonce_valid:uint64 -> r_q:felem -> s_q:felem -> Stack bool
+val check_signature {| cp:S.curve_params |} {| curve_constants |} {| curve_inv_sqrt |} {| PP.precomp_tables |}:
+  are_sk_nonce_valid:uint64 -> r_q:felem -> s_q:felem -> Stack bool
   (requires fun h ->
     live h r_q /\ live h s_q /\ disjoint r_q s_q /\
     (v are_sk_nonce_valid = ones_v U64 \/ v are_sk_nonce_valid = 0))
   (ensures fun h0 res h1 -> modifies0 h0 h1 /\
     res == ((v are_sk_nonce_valid = ones_v U64) && (0 < as_nat h0 r_q) && (0 < as_nat h0 s_q)))
 
-let check_signature {| cp:S.curve_params |} {| PP.precomp_tables |} are_sk_nonce_valid r_q s_q =
+let check_signature {| cp:S.curve_params |} {| curve_constants |} {| curve_inv_sqrt |} {| PP.precomp_tables |} are_sk_nonce_valid r_q s_q =
   let h0 = ST.get () in
   let is_r_zero = bn_is_zero_mask r_q in
   let is_s_zero = bn_is_zero_mask s_q in
@@ -134,9 +137,8 @@ let check_signature {| cp:S.curve_params |} {| PP.precomp_tables |} are_sk_nonce
   BB.unsafe_bool_of_limb m
 
 
-val ecdsa_sign_msg_as_qelem:
-    {| cp:S.curve_params |} -> {| PP.precomp_tables |}
-  -> signature:lbuffer uint8 (2ul *. size cp.bytes)
+val ecdsa_sign_msg_as_qelem {| cp:S.curve_params |} {| curve_constants |} {| curve_inv_sqrt |} {| PP.precomp_tables |}:
+    signature:lbuffer uint8 (2ul *. size cp.bytes)
   -> m_q:felem
   -> private_key:lbuffer uint8 (size cp.bytes)
   -> nonce:lbuffer uint8 (size cp.bytes) ->
@@ -152,7 +154,7 @@ val ecdsa_sign_msg_as_qelem:
      (flag <==> Some? sgnt) /\ (flag ==> (as_seq h1 signature == Some?.v sgnt))))
 
 [@CInline]
-let ecdsa_sign_msg_as_qelem {| cp:S.curve_params |} {| PP.precomp_tables |} signature m_q private_key nonce =
+let ecdsa_sign_msg_as_qelem {| cp:S.curve_params |} {| curve_constants |} {| curve_inv_sqrt |} {| PP.precomp_tables |} signature m_q private_key nonce =
   push_frame ();
   let rsdk_q = create (4ul *. cp.bn_limbs) (u64 0) in
   let r_q = sub rsdk_q 0ul cp.bn_limbs in
