code/nist-pcurves/Hacl.Impl.PCurves.Verify.fst
@@ -9,6 +9,8 @@ open Lib.IntTypes
 open Lib.Buffer
 
 open Hacl.Impl.PCurves.Bignum
+open Hacl.Impl.PCurves.Constants
+open Hacl.Impl.PCurves.InvSqrt
 open Hacl.Impl.PCurves.Point
 open Hacl.Impl.PCurves.Scalar
 open Hacl.Impl.PCurves.PointMul
@@ -26,7 +28,8 @@ module PP = Hacl.PCurves.PrecompTable
 inline_for_extraction noextract
 let lbytes len = lbuffer uint8 len
 
-val qmul_mont: {| c:S.curve_params |} -> sinv:felem -> b:felem -> res:felem -> Stack unit
+val qmul_mont {| c:S.curve_params |} {| curve_constants |} {| curve_inv_sqrt|}:
+  sinv:felem -> b:felem -> res:felem -> Stack unit
   (requires fun h ->
     live h sinv /\ live h b /\ live h res /\
     disjoint sinv res /\ disjoint b res /\
@@ -36,7 +39,7 @@ val qmul_mont: {| c:S.curve_params |} -> sinv:felem -> b:felem -> res:felem -> S
     as_nat h1 res = (as_nat h0 sinv * SM.from_qmont (as_nat h0 b) * SM.qmont_R_inv) % S.order)
 
 [@CInline]
-let qmul_mont {| cp:S.curve_params |} sinv b res =
+let qmul_mont {| cp:S.curve_params |} {| curve_constants |} {| curve_inv_sqrt|} sinv b res =
   let h0 = ST.get () in
   push_frame ();
   let tmp = create_felem #cp in
@@ -50,7 +53,8 @@ let qmul_mont {| cp:S.curve_params |} sinv b res =
 
 
 inline_for_extraction noextract
-val ecdsa_verification_get_u12: {| c:S.curve_params |} -> u1:felem -> u2:felem -> r:felem -> s:felem -> z:felem -> Stack unit
+val ecdsa_verification_get_u12 {| c:S.curve_params |} {| curve_constants |} {| curve_inv_sqrt|}:
+  u1:felem -> u2:felem -> r:felem -> s:felem -> z:felem -> Stack unit
   (requires fun h ->
     live h r /\ live h s /\ live h z /\ live h u1 /\ live h u2 /\
     disjoint u1 u2 /\ disjoint u1 z /\ disjoint u1 r /\ disjoint u1 s /\
@@ -61,11 +65,11 @@ val ecdsa_verification_get_u12: {| c:S.curve_params |} -> u1:felem -> u2:felem -
     as_nat h1 u1 == sinv * as_nat h0 z % S.order /\
     as_nat h1 u2 == sinv * as_nat h0 r % S.order))
 
-let ecdsa_verification_get_u12 {| cp:S.curve_params |} u1 u2 r s z =
+let ecdsa_verification_get_u12 {| cp:S.curve_params |} {| curve_constants |} {| curve_inv_sqrt|} u1 u2 r s z =
   push_frame ();
   let h0 = ST.get () in
   let sinv = create_felem #cp in
-  QI.qinv sinv s;
+  qinv sinv s;
   let h1 = ST.get () in
   assert (qmont_as_nat h1 sinv == S.qinv (qmont_as_nat h0 s));
   //assert (as_nat h2 sinv * SM.qmont_R_inv % S.order ==
@@ -79,7 +83,8 @@ let ecdsa_verification_get_u12 {| cp:S.curve_params |} u1 u2 r s z =
 
 
 inline_for_extraction noextract
-val ecdsa_verify_finv: {| cp:S.curve_params |} -> p:point -> r:felem -> Stack bool
+val ecdsa_verify_finv {| cp:S.curve_params |} {| curve_constants |} {| curve_inv_sqrt|}:
+  p:point -> r:felem -> Stack bool
   (requires fun h ->
     live h p /\ live h r /\ disjoint p r /\
     point_inv h p /\ 0 < as_nat h r /\ as_nat h r < S.order)
@@ -99,7 +104,8 @@ let ecdsa_verify_finv {| cp:S.curve_params |} p r_q =
 
 
 inline_for_extraction noextract
-val ecdsa_verification_cmpr: {| cp:S.curve_params |} -> {| PP.precomp_tables |} -> r:felem -> pk:point -> u1:felem -> u2:felem -> Stack bool
+val ecdsa_verification_cmpr {| cp:S.curve_params |} {| curve_constants |} {| curve_inv_sqrt|} {| PP.precomp_tables |}:
+  r:felem -> pk:point -> u1:felem -> u2:felem -> Stack bool
   (requires fun h ->
     live h r /\ live h pk /\ live h u1 /\ live h u2 /\
     disjoint r u1 /\ disjoint r u2 /\ disjoint r pk /\
@@ -112,7 +118,7 @@ val ecdsa_verification_cmpr: {| cp:S.curve_params |} -> {| PP.precomp_tables |} 
     b <==> (if S.is_point_at_inf (_X, _Y, _Z) then false
       else S.fmul _X (S.finv _Z) % S.order = as_nat h0 r)))
 
-let ecdsa_verification_cmpr {| cp:S.curve_params |} {| PP.precomp_tables |} r pk u1 u2 =
+let ecdsa_verification_cmpr {| cp:S.curve_params |} {| curve_constants |} {| curve_inv_sqrt|} {| PP.precomp_tables |} r pk u1 u2 =
   push_frame ();
   let res = create_point #cp in
   let h0 = ST.get () in
@@ -135,7 +141,7 @@ let ecdsa_verification_cmpr {| cp:S.curve_params |} {| PP.precomp_tables |} r pk
 
 
 inline_for_extraction noextract
-val load_signature {| cp:S.curve_params |} (r_q s_q:felem) (sign_r sign_s:lbytes (size cp.bytes)) : Stack bool
+val load_signature {| cp:S.curve_params |} {| curve_constants |} {| curve_inv_sqrt|} (r_q s_q:felem) (sign_r sign_s:lbytes (size cp.bytes)) : Stack bool
   (requires fun h ->
     live h sign_r /\ live h sign_s /\ live h r_q /\ live h s_q /\
     disjoint r_q s_q /\ disjoint r_q sign_r /\ disjoint r_q sign_s /\
@@ -146,7 +152,7 @@ val load_signature {| cp:S.curve_params |} (r_q s_q:felem) (sign_r sign_s:lbytes
     as_nat h1 r_q = r_q_nat /\ as_nat h1 s_q = s_q_nat /\
     res == (0 < r_q_nat && r_q_nat < S.order && 0 < s_q_nat && s_q_nat < S.order)))
 
-let load_signature {| cp:S.curve_params |} r_q s_q sign_r sign_s =
+let load_signature {| cp:S.curve_params |} {| curve_constants |} {| curve_inv_sqrt|} r_q s_q sign_r sign_s =
   bn_from_bytes_be r_q sign_r;
   bn_from_bytes_be s_q sign_s;
   let is_r_valid = bn_is_lt_order_and_gt_zero_mask r_q in
@@ -155,7 +161,7 @@ let load_signature {| cp:S.curve_params |} r_q s_q sign_r sign_s =
   Hacl.Bignum.Base.unsafe_bool_of_limb is_s_valid
 
 
-val ecdsa_verify_msg_as_qelem {| cp:S.curve_params |} {| PP.precomp_tables |} :
+val ecdsa_verify_msg_as_qelem {| cp:S.curve_params |} {| curve_constants |} {| curve_inv_sqrt|} {| PP.precomp_tables |} :
     m_q:felem
   -> public_key:lbuffer uint8 (2ul *. size cp.bytes)
   -> signature_r:lbuffer uint8 (size cp.bytes)
@@ -169,7 +175,7 @@ val ecdsa_verify_msg_as_qelem {| cp:S.curve_params |} {| PP.precomp_tables |} :
       (as_seq h0 public_key) (as_seq h0 signature_r) (as_seq h0 signature_s))
 
 [@CInline]
-let ecdsa_verify_msg_as_qelem {| cp:S.curve_params |} {| PP.precomp_tables |} m_q public_key signature_r signature_s =
+let ecdsa_verify_msg_as_qelem {| cp:S.curve_params |} {| curve_constants |} {| curve_inv_sqrt|} {| PP.precomp_tables |} m_q public_key signature_r signature_s =
   push_frame ();
   assert (v (3ul *. cp.bn_limbs) == 3 * v cp.bn_limbs);
   assert (v (4ul *. cp.bn_limbs) == 4 * v cp.bn_limbs);
