code/nist-pcurves/Hacl.Impl.PCurves.Compression.fsti
@@ -7,6 +7,8 @@ module ST = FStar.HyperStack.ST
 
 open Lib.IntTypes
 open Lib.Buffer
+open Hacl.Impl.PCurves.Constants
+open Hacl.Impl.PCurves.InvSqrt
 
 module S = Spec.PCurves
 
@@ -22,8 +24,9 @@ val uncompressed_to_raw: {| cp:S.curve_params |} -> pk:lbuffer uint8 (1ul +. 2ul
 
 
 inline_for_extraction noextract
-val compressed_to_raw: {| cp:S.curve_params |} -> pk:lbuffer uint8 (1ul +. size cp.bytes) ->
-                       pk_raw:lbuffer uint8 (2ul *. size cp.bytes) -> Stack bool
+val compressed_to_raw {| cp:S.curve_params |} {| curve_constants |} {| curve_inv_sqrt|}:
+  pk:lbuffer uint8 (1ul +. size cp.bytes) ->
+  pk_raw:lbuffer uint8 (2ul *. size cp.bytes) -> Stack bool
   (requires fun h -> live h pk /\ live h pk_raw /\ disjoint pk pk_raw)
   (ensures  fun h0 b h1 -> modifies (loc pk_raw) h0 h1 /\
     (b <==> Some? (S.pk_compressed_to_raw (as_seq h0 pk))) /\
@@ -31,16 +34,18 @@ val compressed_to_raw: {| cp:S.curve_params |} -> pk:lbuffer uint8 (1ul +. size 
 
 
 inline_for_extraction noextract
-val raw_to_uncompressed: {| cp:S.curve_params |} -> pk_raw:lbuffer uint8 (2ul *. size cp.bytes) ->
-                         pk:lbuffer uint8 (1ul +. 2ul *. size cp.bytes) -> Stack unit
+val raw_to_uncompressed {| cp:S.curve_params |} {| curve_constants |} {| curve_inv_sqrt|}:
+  pk_raw:lbuffer uint8 (2ul *. size cp.bytes) ->
+  pk:lbuffer uint8 (1ul +. 2ul *. size cp.bytes) -> Stack unit
   (requires fun h -> live h pk /\ live h pk_raw /\ disjoint pk pk_raw)
   (ensures fun h0 _ h1 -> modifies (loc pk) h0 h1 /\
     as_seq h1 pk == S.pk_uncompressed_from_raw (as_seq h0 pk_raw))
 
 
 inline_for_extraction noextract
-val raw_to_compressed: {| cp:S.curve_params |} -> pk_raw:lbuffer uint8 (2ul *. size cp.bytes) ->
-                       pk:lbuffer uint8 (1ul +. size cp.bytes) -> Stack unit
+val raw_to_compressed {| cp:S.curve_params |} {| curve_constants |} {| curve_inv_sqrt|}:
+  pk_raw:lbuffer uint8 (2ul *. size cp.bytes) ->
+  pk:lbuffer uint8 (1ul +. size cp.bytes) -> Stack unit
   (requires fun h -> live h pk /\ live h pk_raw /\ disjoint pk pk_raw)
   (ensures  fun h0 _ h1 -> modifies (loc pk) h0 h1 /\
     as_seq h1 pk == S.pk_compressed_from_raw (as_seq h0 pk_raw))
