code/nist-pcurves/Hacl.Impl.PCurves.PointMul.fsti
@@ -9,6 +9,8 @@ open Lib.IntTypes
 open Lib.Buffer
 
 open Hacl.Impl.PCurves.Bignum
+open Hacl.Impl.PCurves.Constants
+open Hacl.Impl.PCurves.InvSqrt
 open Hacl.Impl.PCurves.Point
 
 module S = Spec.PCurves
@@ -19,7 +21,8 @@ include Hacl.PCurves.PrecompTable
 
 #set-options "--z3rlimit 30 --fuel 0 --ifuel 0"
 
-val point_mul: {| cp:S.curve_params |} -> {| pt:precomp_tables |} -> res:point -> scalar:felem -> p:point -> Stack unit
+val point_mul {| cp:S.curve_params |} {| curve_constants |} {| curve_inv_sqrt|} {| pt:precomp_tables |}:
+  res:point -> scalar:felem -> p:point -> Stack unit
   (requires fun h ->
     live h p /\ live h res /\ live h scalar /\
     disjoint p res /\ disjoint scalar res /\ disjoint p scalar /\
@@ -30,7 +33,8 @@ val point_mul: {| cp:S.curve_params |} -> {| pt:precomp_tables |} -> res:point -
     S.to_aff_point (S.point_mul (as_nat h0 scalar) (from_mont_point (as_point_nat h0 p))))
 
 
-val point_mul_g: {| cp:S.curve_params |} -> {| pt:precomp_tables |} -> res:point -> scalar:felem -> Stack unit
+val point_mul_g {| cp:S.curve_params |} {| curve_constants |} {| curve_inv_sqrt|} {| pt:precomp_tables |}:
+  res:point -> scalar:felem -> Stack unit
   (requires fun h ->
     live h res /\ live h scalar /\ disjoint res scalar /\
     as_nat h scalar < S.order)
@@ -40,7 +44,8 @@ val point_mul_g: {| cp:S.curve_params |} -> {| pt:precomp_tables |} -> res:point
     S.to_aff_point (S.point_mul_g (as_nat h0 scalar)))
 
 
-val point_mul_double_g: {| cp:S.curve_params |} -> {| pt:precomp_tables |} -> res:point -> scalar1:felem -> scalar2:felem -> p:point -> Stack unit
+val point_mul_double_g {| cp:S.curve_params |} {| curve_constants |} {| curve_inv_sqrt|} {| pt:precomp_tables |}:
+  res:point -> scalar1:felem -> scalar2:felem -> p:point -> Stack unit
   (requires fun h ->
     live h res /\ live h scalar1 /\ live h scalar2 /\ live h p /\
     disjoint res scalar1 /\ disjoint res scalar2 /\ disjoint res p /\
